porting changes to paths

src/extensions/paths-new/OperationalSemantics.v
@@ -1,309 +1,51 @@
 Set Implicit Arguments.
 
-Require Import List Coq.Program.Equality.
+Require Import Coq.Program.Equality.
 Require Import LibLN.
 Require Import Definitions Binding.
 
-(** * Normal Forms
-A normal form is defined in the WadlerFest DOT paper as:
+(** * Stack-Based Operational Semantics *)
 
-[n ::= x | v | let x = v in n]
+Reserved Notation "t1 '|->' t2" (at level 40, t2 at level 39).
 
-This corresponds to an evaluation context of the form
-[(let x = v in)* [ ]] whose hole is filled by a variable [x]
-or value [v]. *)
+Inductive red : sta * trm -> sta * trm -> Prop :=
+(** [s(x) = lambda(T)t]      #<br>#
+    [―――――――――――――――――――――]  #<br>#
+    [(s, x y) |-> (s, t^y)]  *)
+| red_sel : forall x m s t T ds,
+    binds x (val_new T ds) s ->
+    defs_has (open_defs x ds) (def_trm m t) ->
+    (s, trm_sel (avar_f x) m) |-> (s, t)
 
-Inductive normal_form: trm -> Prop :=
-| nf_var: forall p, normal_form (trm_path p)
-| nf_val: forall v, normal_form (trm_val v)
-| nf_let: forall v t, normal_form t -> normal_form (trm_let (trm_val v) t).
+(** [s(x) = nu(T)...{a = t}...]  #<br>#
+    [―――――――――――――――――――――――――]  #<br>#
+    [(s, x.a) |-> (s, t)      ]  *)
+| red_app : forall f a s T t,
+    binds f (val_lambda T t) s ->
+    (s, trm_app (avar_f f) (avar_f a)) |-> (s, open_trm a t)
 
-Hint Constructors normal_form.
+(** [(s, let x = v in t) |-> ((s, x = v), t^x)] *)
+| red_let : forall v t s x,
+    x # s ->
+    (s, trm_let (trm_val v) t) |-> (s & x ~ v, open_trm x t)
 
-(** * Operational Semantics
+(** [(s, let y = x in t) |-> (s, t^x)] *)
+| red_let_var : forall t s x,
+    (s, trm_let (trm_var (avar_f x)) t) |-> (s, open_trm x t)
 
-The first four reduction rules correspond directly to the rules in Figure 7 of the paper.
+(** [(s, t0) |-> (s', t0')]                             #<br>#
+    [―――――――――――――――――――――――――――――――――――――――――――――――]  #<br>#
+    [(s, let x = t0 in t) |-> (s', let x = t0' in t)]  *)
+| red_let_tgt : forall t0 t s t0' s',
+    (s, t0) |-> (s', t0') ->
+    (s, trm_let t0 t) |-> (s', trm_let t0' t)
 
-The last two rules are congruence rules that implement the meaning of evaluation contexts.
-Specifically, if a term [u] decomposes into an evaluation context and subterm
-as [u = e[t]] and [e[t]] reduces to [e[t']] according to the rules from Figure 7,
-then the purpose of the two congruence rules is to ensure that [u] also reduces
-to [u'], where [u'] is the term [u' = e[t']]. The grammar for evaluation contexts
-in the paper is:
+where "t1 '|->' t2" := (red t1 t2).
 
-[e ::= [] | let x = [] in t | let x = v in e]
+(** ** Normal forms *)
+(** Variables and values are considered to be in normal form. *)
+Inductive norm_form: trm -> Prop :=
+| nf_var: forall x, norm_form (trm_var x)
+| nf_val: forall v, norm_form (trm_val v).
 
-A sentential form [eta] in a derivation of an evaluation context [e] is a string
-of terminals (the elements of DOT terms) and the non-terminal [e]. Define
-[e(eta)] to be a string of terminals formed by replacing [e] with [[]] in [eta].
-We argue that whenever [eta_1] directly derives [eta_2] ([eta_1 => eta_2]),
-and the reduction rules infer that [e(eta_2)[t_2] |-> e(eta_2)[t_2']], then the
-reduction rules also infer that [e(eta_1)[t_1] |-> e(eta_1)[t_1']], where
-[e(eta_2)[t_2] = e(eta_1)[t_1]] and [e(eta_2)[t_2'] = e(eta_1)[t_1']].
-The argument is by considering each of the three cases
-in the evaluation context grammar that justify [eta_1 => eta_2].
-The first case replaces [e] with [[]], so [e(eta_1) = e(eta_2)], so the conclusion
-trivially holds. The second case replaces [e] with [let x = [] in t]. In this case,
-the reduction congruence rule [red_let_trm] has [e(eta_2)[t_2] |-> e(eta_2)[t_2']]
-as a premise and [e(eta_1)[t_1] |-> e(eta_1)[t_1']] as a conclusion. The third case
-replaces [e] with [let x = v in e].  Similarly, the congruence rule [red_let_val]
-has [e(eta_2)[t_2] |-> e(eta_2)[t_2']] as a premise and [e(eta_1)[t_1] |-> e(eta_1)[t_1']]
-as a conclusion. Thus, whenever [eta_1 => eta_2] and [e(eta_2)[t_2] |-> e(eta_2)[t_2']],
-we also have that [e(eta_1)[t_1] |-> e(eta_1)[t_1']].
-
-Reasoning inductively about the steps in the context-free grammar derivation of [e],
-for every sentential
-form [eta] that occurs in that derivation, the congruence reduction rules infer that
-[e(eta)[u] |-> e(eta)[u']], where
-[e(eta)[u] = e[t]] and [e(eta)[u'] = e[t']]. In particular, this is true for the
-sentential form [eta = e], the first sentential form of every derivation. Since
-[e(eta) = e(e) = []], we have shown that the congruence reduction rules infer that [u |-> u'].
-
-Starting with an evaluation context [e] in its conclusion, the [red_let_val] rule appends
-[let x = v] to the context to yield a new context used in its premise.
-(More precisely, the rule replaces the non-terminal [e] within the context in the conclusion by
-[let x = v in e].) This is the only reduction rule that modifies an existing evaluation context. Therefore,
-in a derivation of a reduction judgment [u |-> u'] in an empty evaluation context, every evaluation context
-that appears in the derivation is of the form [let x_1 = v_1 in ... let x_n = v_n in []].
-Therefore, in order to be able to represent every step of every such derivation of a reduction
-judgement in the Coq proof, it is sufficient to represent evaluation contexts by a data structure
-that can represent all evaluation contexts of this form. The proof represents these evaluation
-contexts by a list of pairs of variables and values.
-*)
-
-Reserved Notation "e '[' t1 '|->' t2 ']'" (at level 60, t1 at level 39).
-
-Inductive red : ec -> trm -> trm -> Prop :=
-
-(** [e(x) = lambda(T)t]     #<br>#
-    [――――――――――――――――――――]  #<br>#
-    [e[x y] |-> e[t^y] ]  *)
-| red_apply : forall e p q T t,
-    lc_trm (trm_app p q) ->
-    e ∋ (p, val_lambda T t) ->
-    e [ trm_app p q |-> open_trm_p q t ]
-
-(** [e[let x = p in t] |-> e[t^p]] *)
-| red_let_var : forall p t e,
-    lc_trm (trm_let (trm_path p) t) ->
-    e [ trm_let (trm_path p) t |-> open_trm_p p t ]
-
-(** [e[let x = (let y = s in t) in u] |-> e[let y = s in let x = t in u]] *)
-| red_let_let : forall s t u e,
-    lc_trm (trm_let (trm_let s t) u) ->
-    e [ trm_let (trm_let s t) u |-> trm_let s (trm_let t u) ]
-
-(** [e[t] |-> e[t']]                            #<br>#
-    [――――――――――――――――――――――――――――――――――――――――]  #<br>#
-    [e[let x = t in u] |-> e[let x = t' in u]]     *)
-| red_let_trm : forall e t t' u,
-    lc_trm (trm_let t u) ->
-    e [ t |-> t' ] ->
-    e [ trm_let t u |-> trm_let t' u ]
-
-(** [(e, x = v) [t] |-> (e, x = v) [t']]        #<br>#
-    [――――――――――――――――――――――――――――――――――――――――]   #<br>#
-    [e[let x = v in t] |-> e[let x = v in t']]   *)
-| red_let_val: forall e t t' v L,
-    lc_trm (trm_let (trm_val v) t) ->
-    (forall x, x \notin L  ->
-      (e & x ~ v) [ open_trm x t |-> open_trm x t' ]) ->
-    e [ trm_let (trm_val v) t |-> trm_let (trm_val v) t' ]
-
-where "e [ t |-> t' ]" := (red e t t').
-
-Hint Constructors red normal_form.
-
-(** Reduction in an empty context *)
-Notation "t '|->' u" := (empty [t |-> u]) (at level 50).
-
-(** Typing in an empty context *)
-Notation "'⊢' t ':' T" := (empty ⊢ t: T) (at level 40, t at level 59).
-
-(** If [e] is locally closed and [e[t] |-> e[t']], then [t'] is locally closed.  *)
-Lemma lc_env_eval_to_lc_trm : forall e t t',
-    lc_ec e ->
-    e [t |-> t'] ->
-    lc_trm t'.
-Proof with auto.
-  introv Hlce He.
-  induction He;
-    match goal with
-    | [ H : lc_at_trm _ _ |- _ ] => inversions H
-    end;
-    repeat constructor;
-    do 2 try
-       match goal with
-       | [ H : binds _ _ _ |- _ ] => apply lc_ec_binds_inv in H; eauto
-       | [ H : lc_at_val _ _ |- _ ] => inversions H
-       | [ H : lc_at_trm _ _ |- _ ] => solve [inversions H; auto]
-       end;
-    try applys lc_at_to_open_trm_val_def_defs;
-    eauto.
-Admitted. (*  - apply lc_defs_has in H1... inversion H1...
-    applys lc_at_to_open_trm_val_def_defs...
-  - eapply lc_at_relaxing_trm_val_def_defs; try eassumption.
-    omega.
-  - inversion H4. pick_fresh x.
-    assert (x \notin L); auto.
-    assert (lc_ec (e & x ~ v)); auto.
-    specialize (H1 x H3 H6).
-    applys open_to_lc_at_trm_val_def_defs. eassumption.
-Qed.*)
-
-(** The next two lemmas show that if [t^x] is in normal form, then [t] is in normal form. *)
-Lemma open_rec_preserve_normal_form: forall k x t,
-    x \notin fv_trm t ->
-    normal_form (open_rec_trm k x t) ->
-    normal_form t.
-Proof.
-  intros. generalize dependent x.
-  generalize dependent k.
-  induction t; auto; intros;
-    try solve [
-    unfold open_trm in H0; unfold open_rec_trm in H0;
-    inversion H0].
-  unfold open_trm in H0. unfold open_rec_trm in H0.
-  inversion H0. fold open_rec_trm in *.
-  unfold fv_trm in H. fold fv_trm in H.
-  assert (x \notin fv_trm t2); auto.
-  specialize (IHt2 _ _ H4 H2).
-
-  destruct t1; simpl; inversion H1.
-  constructor. auto.
-Qed.
-
-(** See previous lemma [open_rec_preserve_normal_form]. *)
-Lemma open_preserve_normal_form : forall x t,
-    x \notin fv_trm t ->
-    normal_form (open_trm x t) ->
-    normal_form t.
-Proof.
-  apply open_rec_preserve_normal_form.
-Qed.
-
-(** [x] fresh                            #<br>#
-    [e] and [v] are locally closed       #<br>#
-    [(e, x=v)[t^x] |-> (e, x=v)[t']]     #<br>#
-    [――――――――――――――――――――――――――――――――――] #<br>#
-    [exists f. x \notin fv(f) and t' = f^x    *)
-Lemma open_rec_eval_to_open_rec : forall e x t t' v,
-    x \notin dom e \u fv_trm t \u fv_val v ->
-    lc_ec e -> lc_val v ->
-    e & x ~ v[ open_trm x t |-> t'] ->
-    exists f, (x \notin (fv_trm f)) /\ t' = open_trm x f.
-Proof.
-  intros. exists (close_trm x t'). remember (close_trm x t') as ct. split.
-  - subst ct. apply close_rec_trm_val_def_defs_no_capture.
-  - symmetry. rewrite Heqct. apply open_left_inverse_close_trm_val_def_defs.
-    eauto using lc_env_eval_to_lc_trm, lc_ec_cons.
-Qed.
-
-(** Substitution for reduction *)
-
-(** [x, y] fresh                                                  #<br>#
-    [(e1, x=v, e2)[t1] |-> (e1, x=v, e2)[t2]]                     #<br>#
-    [―――――――――――――――――――――――――――――――――――――――――――――――――――――――――――] #<br>#
-    [(e1, y=v[y/x], e2)[t1[y/x]] |-> (e1, y=v[y/x], e2)[t2[y/x]]] *)
-(*Lemma eval_renaming_subst : forall x y e1 e2 v t1 t2,
-    x \notin dom e1 \u fv_ec_vals e1 \u dom e2 ->
-    y \notin dom e1 \u fv_ec_vals e1
-      \u dom e2 \u fv_ec_vals e2 \u fv_val v \u fv_trm t1 ->
-    (e1 & x ~ v & e2)[t1 |-> t2] ->
-    (e1 & y ~ subst_val x y v & subst_env x y e2)[subst_trm x y t1 |-> subst_trm x y t2].
-Proof.
-  Local Hint Resolve binds_subst_env.
-
-  Local Ltac contra_bind :=
-    repeat match goal with
-           | [ H : _ \notin _ \u _ |- _ ] => apply notin_union in H; destruct H
-           end;
-    match goal with
-    | [ _ : ?x \notin dom ?e, _ : binds ?x _ ?e |- _ ] =>
-      exfalso; eapply binds_fresh_inv; [eassumption | auto 1]
-    end.
-
-  Local Ltac solve_left_most :=
-    apply binds_concat_left; unfold subst_env; try rewrite dom_map;
-    try rewrite (proj1 (proj2 (subst_fresh_trm_val_def_defs _ _))); auto;
-    eapply binds_fv_ec_vals; eauto 2.
-
-  introv Hfx Hfy He. dependent induction He; simpls.
-  - apply binds_middle_inv in H0; destruct_all; case_if; subst;
-      try contra_bind;
-      rewrite subst_open_commut_trm; unfold subst_fvar; case_if;
-        apply red_apply with (subst_typ x y T);
-          assert (Hs : val_lambda (subst_typ x y T) (subst_trm x y t) =
-                       subst_val x y (val_lambda T t)) by auto;
-          auto 2;
-          rewrite Hs;
-          try match goal with
-              | [ |- binds ?y _ (_ & ?y ~ _ & _) ] =>
-                apply binds_middle_eq; unfold subst_env; rewrite dom_map; auto 1
-              end;
-          try solve [apply binds_concat_right, binds_subst_env; trivial];
-          solve_left_most.
-  - apply binds_middle_inv in H0; destruct_all; case_if; subst;
-      try contra_bind;
-      apply red_project with (T:=subst_typ x y T) (ds:=subst_defs x y ds); auto 1;
-        assert (Hs : val_new (subst_typ x y T) (subst_defs x y ds) = subst_val x y (val_new T ds));
-        auto 2;
-        try rewrite Hs.
-    + apply binds_concat_right; apply binds_subst_env; trivial.
-    + apply open_subst_defs; auto.
-    + apply binds_middle_eq; unfold subst_env; rewrite dom_map; auto.
-    + apply open_subst_defs2; auto.
-    + solve_left_most.
-    + apply open_subst_defs; auto.
-  - case_if; simpls;
-      subst; rewrite subst_open_commut_trm; unfold subst_fvar;
-        case_if; constructor;
-          inversion H; constructor; auto;
-            apply lc_at_subst_trm_val_def_defs; trivial.
-  - inversion H. inversion H2.
-    repeat constructor; auto;
-      apply lc_at_subst_trm_val_def_defs; trivial.
-  - inversion H.
-    repeat constructor; auto;
-      apply lc_at_subst_trm_val_def_defs; trivial.
-  - econstructor.
-    + inversion H. inversion H4.
-      repeat constructor;
-        apply lc_at_subst_trm_val_def_defs; trivial.
-    + intros.
-      instantiate (1 := L \u dom e1 \u fv_ec_vals e1 \u dom e2 \u fv_ec_vals e2
-                            \u fv_val v \u fv_val v0 \u fv_trm t \u \{x} \u \{y}) in H2.
-
-      assert (x0 <> x) by auto.
-      assert (x0 <> y) by auto.
-
-      assert (subst_fvar x y x0 = x0). {
-        unfold subst_fvar. case_if; auto.
-      }
-      rewrite <- H5.
-      rewrite <- subst_open_commut_trm. rewrite <- subst_open_commut_trm.
-      rewrite H5.
-
-      assert (x0 \notin L) by auto.
-      specialize (H1 _ H6 v (e2 & x0 ~ v0) e1).
-
-      assert (y \notin fv_trm (open_trm x0 t)). {
-        apply open_fv_trm_val_def_defs; auto.
-      }
-      assert (y \notin fv_ec_vals (e2 & x0 ~ v0)) by rewrite~ fv_ec_vals_push_eq.
-
-      assert (y \notin dom e1 \u fv_ec_vals e1
-                \u dom (e2 & x0 ~ v0) \u fv_ec_vals (e2 & x0 ~ v0)
-                \u fv_val v \u fv_trm (open_trm x0 t)); auto.
-
-      assert (x \notin dom e1 \u fv_ec_vals e1 \u dom (e2 & x0 ~ v0)); auto.
-
-      assert (subst_env x y (e2 & x0 ~ v0) = subst_env x y e2 & x0 ~ subst_val x y v0). {
-        unfold subst_env. apply map_push.
-      }
-      specialize (H1 H9 _ H10).
-      rewrite H11 in H1.
-      rewrite? concat_assoc in H1.
-      apply H1. auto.
-Qed.
- *)
+Hint Constructors red norm_form.
