src/extensions/paths-new/Safety.v
@@ -1,20 +1,24 @@
-(** printing ⊢#    %\vdash_{\#}%    #&vdash;<sub>&#35;</sub>#     *)
-(** printing ⊢##   %\vdash_{\#\#}%  #&vdash;<sub>&#35&#35</sub>#  *)
-(** printing ⊢##v  %\vdash_{\#\#v}% #&vdash;<sub>&#35&#35v</sub># *)
-(** printing ⊢!    %\vdash_!%       #&vdash;<sub>!</sub>#         *)
-(** remove printing ~ *)
-
 Set Implicit Arguments.
 
-Require Import Coq.Program.Equality.
 Require Import LibLN.
-Require Import Definitions.
-Require Import RecordAndInertTypes.
-Require Import Binding.
-Require Import OperationalSemantics.
-Require Import Weakening SubEnvironments Narrowing PreciseTypes Substitution CanonicalForms.
+Require Import Coq.Program.Equality.
+Require Import Definitions Weakening Narrowing Binding PreciseTypes Substitution CanonicalForms
+        RecordAndInertTypes InvertibleTypes GeneralToTight OperationalSemantics.
 
-(** * Progress *)
+(** For the purposes of our evaluation semantics, a term is a
+ The typing of a term with a stack *)
+Inductive sta_trm_typ : sta * trm -> typ -> Prop :=
+| sta_trm_typ_c : forall G s t T,
+    inert G ->
+    well_typed G s ->
+    G ⊢ t : T ->
+    sta_trm_typ (s, t) T.
+
+Hint Constructors sta_trm_typ.
+
+Notation "'⊢' t ':' T" := (sta_trm_typ t T) (at level 40, t at level 59).
+
+(** * Preservation *)
 
 (** If a value [v] has type [T], then [v] has a precise type [T']
     that is a subtype of [T].
@@ -25,286 +29,156 @@ Lemma val_typing: forall G v T,
         G ⊢ T' <: T.
 Proof.
   intros G v T H. dependent induction H; eauto.
-  destruct (IHty_trm _ eq_refl) as [T' [Hty Hsub]]. eauto.
+  destruct (IHty_trm _ eq_refl). destruct_all. eauto.
 Qed.
 
-(** [e] and [t] are locally closed          #<br>#
-    [G' ⪯ G]                                #<br>#
-    inert [G']                              #<br>#
-    [e: G']                                 #<br>#
-    [G ⊢ t: T]                              #<br>#
-    [―――――――――――――――――――――――――――――]         #<br>#
-    [t] is in normal form or [e[t] |-> e[t']] *)
-Lemma progress_ec: forall G' G e t T,
-    lc_ec e ->
-    lc_trm t ->
-    G' ⪯ G ->
-    inert G' ->
-    wf_sto G' e ->
-    G ⊢ t: T ->
-    ok G ->
-    (normal_form t \/ exists t', e[t |-> t']).
-Proof with auto.
-  introv Hlce Hlc Hsenv Hig Hwt Ht Hokg. gen G' e.
-  induction Ht; eauto; intros.
-  - Case "ty_var". left. constructor.
-  - Case "ty_all_elim".
-    apply narrow_typing with (G':=G') in Ht1; auto.
-    destruct (canonical_forms_fun Hig Hwt Ht1) as [L [T' [t [Bis [Hsub Hty]]]]].
-    right. repeat eexists. apply* red_apply.
-  - Case "ty_new_elim".
-    apply narrow_typing with (G':=G') in Ht; auto.
-    destruct (canonical_forms_obj Hig Hwt Ht) as [S [ds [t [Bis [Has Ty]]]]].
-    right. repeat eexists. apply* red_project.
-  - Case "ty_let".
-    destruct t.
-    + SCase "t = trm_var a".
-      apply narrow_typing with (G':=G') in Ht; auto.
-      right.
-      assert (var_typing_implies_avar_f: forall G a T, G ⊢ trm_var a : T -> exists x, a = avar_f x)
-        by (introv HGat; dependent induction HGat; eauto).
-      destruct (var_typing_implies_avar_f _ _ _ Ht); subst.
-      exists (open_trm x u). constructor...
-    + SCase "t = trm_val v".
-      apply val_typing in Ht.
-      destruct Ht as [T' [H1 H2]].
-      pose proof (precise_inert_typ H1) as Hpit.
-      pick_fresh x.
-      destruct H0 with (x:=x) (G' := G' & x ~ T') (e := e & x ~ v); auto 2.
-      * inversion Hlc. trivial. apply lc_at_to_open_trm_val_def_defs...
-      * intros. eapply subenv_trans; econstructor; eauto.
-      * constructor; auto. inversion Hlc. inversion H5. trivial.
-      * intros. apply precise_to_general in H1.
-        constructor; auto. eapply narrow_typing in H1; eauto.
-      * left.
-        destruct u; auto; apply open_preserve_normal_form in H3; auto.
-      * right. destruct H3.
-        pose proof H3. inversion Hlc. inversion H7.
-        apply open_rec_eval_to_open_rec in H3; auto.
-        destruct_all. subst.
-        exists (trm_let (trm_val v) x1).
+(** Helper tactics for proving Preservation *)
 
-        apply red_let_val with (L \u dom G \u fv_ctx_types G \u dom G
-                                  \u fv_ctx_types G \u dom e \u fv_ec_vals e
-                                  \u fv_trm (open_trm x u) \u fv_val v \u fv_typ T
-                                  \u fv_typ U \u fv_typ T' \u fv_trm x1
-                                  \u dom (empty : ec) \u fv_ec_vals empty); auto.
-        intros.
+Ltac binds_eq :=
+  match goal with
+  | [Hb1: binds ?x _ ?G,
+     Hb2: binds ?x _ ?G |- _] =>
+     apply (binds_func Hb1) in Hb2; inversions Hb2
+  end.
 
-        replace (e & x ~ v) with (e & x ~ v & empty) in H4;
-          try (rewrite <- concat_empty_r; trivial).
+Ltac invert_red :=
+  match goal with
+  | [Hr: (_, _) |-> (_, _) |- _] => inversions Hr
+  end.
 
+Ltac solve_IH :=
+  match goal with
+  | [IH: well_typed _ _ ->
+         inert _ ->
+         forall t', (_, _) |-> (_, _) -> _,
+       Wf: well_typed _ _,
+       In: inert _,
+       Hr: (_, _) |-> (_, ?t') |- _] =>
+    specialize (IH Wf In t' Hr); destruct_all
+  end;
+  match goal with
+  | [Hi: _ & ?G' ⊢ _ : _ |- _] =>
+    exists G'; repeat split; auto
+  end.
 
-        replace (e & x0 ~ v) with (e & x0 ~ v & empty);
-        try (rewrite <- concat_empty_r; trivial).
+Ltac solve_let :=
+  invert_red; solve_IH; fresh_constructor; eauto; apply* weaken_rules.
 
-        assert (Hsubstv : subst_val x x0 v = v). {
-          apply subst_fresh_trm_val_def_defs. auto.
-        }
-        rewrite <- Hsubstv.
-
-        assert (Hleft : open_trm x0 u = subst_trm x x0 (open_trm x u)). {
-          apply subst_intro_trm. auto.
-        }
-        rewrite Hleft.
-
-        assert (Hright : open_trm x0 x1 = subst_trm x x0 (open_trm x x1)). {
-          apply subst_intro_trm. auto.
-        }
-        rewrite Hright.
-
-        replace empty with (subst_env x x0 empty); try apply map_empty; trivial.
-
-        apply eval_renaming_subst; auto.
-    + SCase "t = trm_sel a t".
-      right.
-      inversion Hlc.
-      destruct (IHHt H3 Hokg G' Hsenv Hig e Hlce Hwt) as [Hnf | [t' Hr]]. inversion Hnf.
-      eexists. constructor*.
-    + SCase "t = trm_app a a0".
-      right.
-      inversion Hlc.
-      destruct (IHHt H3 Hokg G' Hsenv Hig e Hlce Hwt) as [Hnf | [t' Hr]]. inversion Hnf.
-      eexists. constructor*.
-    + SCase "t = trm_let t1 t2".
-      right. eexists. constructor. inversion Hlc. trivial.
-Qed.
-
-(** ** Progress Theorem
-    If [⊢ t : T], then either [t] is a normal form,
-    or [t]] reduces to some [t']. *)
-Theorem progress: forall t T,
-    lc_trm t ->
-    ⊢ t: T ->
-    normal_form t \/ (exists t', t |-> t').
-Proof.
-  intros. apply* progress_ec.
-Qed.
-
-(** * Preservation *)
-
-(** [t] is locally closed   #<br>#
-    [G' ⪯ G]                #<br>#
-    [e: G']                 #<br>#
-    inert [G']              #<br>#
+(** [s: G]                  #<br>#
+    [inert [G]              #<br>#
+    [(s, t) |-> (s', t')]   #<br>#
     [G ⊢ t: T]              #<br>#
-    [e[t] |-> e[t']]        #<br>#
-    [ok G]                  #<br>#
     [―――――――――――――――――――]   #<br>#
-    [G' ⊢ t': T]            *)
-Lemma preservation_ec: forall G G' e t t' T,
-    lc_trm t ->
-    G' ⪯ G ->
-    well_typed G' e ->
-    inert G' ->
-    G ⊢ t: T ->
-    e[t |-> t'] ->
-    ok G ->
-    G' ⊢ t': T.
+    [exists G', inert G']        #<br>#
+    [s': G, G']             #<br>#
+    [G, G' ⊢ t': T]         *)
+Lemma preservation_helper: forall G s t s' t' T,
+    well_typed G s ->
+    inert G ->
+    (s, t) |-> (s', t') ->
+    G ⊢ t : T ->
+    exists G', inert G' /\
+          well_typed (G & G') s' /\
+          G & G' ⊢ t' : T.
 Proof.
-  Local Hint Resolve open_bound_lc_trm.
-  introv Hlc Hsenv Hwt Hi Ht Hr Hok. gen e t'. gen G'.
-  induction Ht; introv Hsenv Hi Hwt Hr; try solve [inversions Hr].
+  introv Hwf Hin Hred Ht. gen t'.
+  dependent induction Ht; intros; try solve [invert_red].
   - Case "ty_all_elim".
-    apply narrow_typing with (G':=G') in Ht1; auto.
-    destruct (canonical_forms_fun Hi Hwt Ht1) as [L [T' [t [Bis [Hsub Hty]]]]].
-    inversions Hr.
-    apply (binds_func H4) in Bis. inversions Bis.
-    pick_fresh y. apply~ renaming_typ.
-    apply (narrow_typing Ht2); auto.
+    match goal with
+    | [Hx: _ ⊢ trm_var (avar_f _) : typ_all _ _ |- _] =>
+        pose proof (canonical_forms_fun Hin Hwf Hx) as [L [T' [t [Bis [Hsub Hty]]]]];
+          inversions Hred;
+          binds_eq
+    end.
+    exists (@empty typ). rewrite concat_empty_r. repeat split; auto.
+    pick_fresh y. assert (y \notin L) as FrL by auto. specialize (Hty y FrL).
+    eapply renaming_typ; eauto.
   - Case "ty_new_elim".
-    apply narrow_typing with (G':=G') in Ht; auto.
-    destruct (canonical_forms_obj Hi Hwt Ht) as [S [ds [t [Bis [Has Ty]]]]].
-    inversions Hr.
-    apply (binds_func H3) in Bis. inversions Bis.
-    rewrite <- (defs_has_inv Has H5). assumption.
+    pose proof (canonical_forms_obj Hin Hwf Ht) as [S [ds [t [Bis [Has Ty]]]]].
+    invert_red. binds_eq.
+    exists (@empty typ). rewrite concat_empty_r. repeat split; auto.
+    match goal with
+    | [Hd: defs_has _ (def_trm _ ?t') |- G ⊢ t': T] =>
+      rewrite* <- (defs_has_inv Has Hd)
+    end.
   - Case "ty_let".
-    inversions Hr.
-    * SCase "red_let_var".
-      pick_fresh x. assert (x \notin L); auto. specialize (H x H1).
-      apply subst_ty_trm with (y:=y) in H; auto.
-      -- assert (subst_typ x y U = U). {
-           apply subst_fresh_typ_dec. auto.
-         }
-         rewrite H2 in H.
-         assert (open_trm y u = subst_trm x y (open_trm x u)). {
-           apply subst_intro_trm. auto.
-         }
-         rewrite <- H3 in H.
-         apply narrow_typing with (G':=G') in H; auto.
-      -- assert (subst_typ x y T = T). {
-           apply subst_fresh_typ_dec. auto.
-         }
-         rewrite H2. trivial.
-    * SCase "red_let_let".
-      clear H0 IHHt.
-      assert (forall x, x \notin (L \u dom G) -> G & x ~ T ⊢ open_trm x u : U). {
-        intros. assert (x \notin L); auto.
-      }
-      clear H.
-      dependent induction Ht.
-      -- apply narrow_typing with (G' := G') in Ht; eauto.
-         remember ((((((((((((L \u L0) \u dom G) \u fv_ctx_types G) \u dom G')
-                            \u fv_ctx_types G') \u dom e) \u fv_trm u) \u fv_trm s)
-                        \u fv_trm t0) \u fv_typ U) \u fv_typ T) \u fv_typ U0) as bigL.
-         econstructor; eauto. intros.
-         instantiate (1 := bigL) in H2.
-         unfold open_trm, open_rec_trm. fold open_rec_trm.
-
-         assert (open_rec_trm 1 x u = u). {
-           inversion H5. apply open_bound_lc_trm.
-           apply lc_at_to_open_trm_val_def_defs. trivial.
-         }
-         rewrite H3. clear H3.
-
-         rewrite HeqbigL in H2.
-         assert (x \notin L0); auto.
-         specialize (H _ H3).
-         assert (G' & x ~ T ⪯ G & x ~ T); auto.
-         apply narrow_typing with (G' := G' & x ~ T) in H; auto.
-         rewrite <- HeqbigL in H2.
-         econstructor; eauto.
-         intros. instantiate (1 := bigL \u \{ x }) in H6.
-         subst bigL.
-         assert (x0 \notin L \u dom G); auto.
-         specialize (H1 _ H7).
-         assert (G' & x0 ~ U0 ⊢ open_trm x0 u : U). {
-           eapply narrow_typing; [eassumption |]; auto.
-         }
-         eapply (proj1 weaken_rules); eauto.
-      -- eapply IHHt; eauto; intros.
-         specialize (H0 _ H1).
-         eapply narrow_typing; eauto.
-    * SCase "red_let_trm".
-      inversion Hlc.
-      specialize (IHHt H3 Hok _ Hsenv Hi _ Hwt t'0 H6).
-      eapply ty_let; eauto. intros.
-      instantiate (1 := (((((((((L \u dom G) \u fv_ctx_types G) \u dom G')
-                                \u fv_ctx_types G') \u dom e) \u fv_trm t) \u fv_trm u)
-                            \u fv_trm t'0) \u fv_typ T) \u fv_typ U) in H7.
-      assert (x \notin L); auto.
-      specialize (H _ H8).
-      apply (narrow_typing H); auto.
-    * SCase "red_let_val".
-      apply val_typing in Ht.
-      destruct Ht as [T' [H1 H2]].
-      pose proof (precise_inert_typ H1) as Hpit.
-      pose proof H1 as Htt.
-      apply precise_to_general in Htt.
-      apply narrow_typing with (G':=G') in Htt; auto.
-      pick_fresh x. assert (x \notin L); auto.
-      assert (ok (G & x ~ T)); auto.
-      assert (G' & x ~ T' ⪯ G & x ~ T). {
-        apply subenv_trans with (G & x ~ T'); auto.
-      }
-      assert (inert (G' & x ~ T')) by auto.
-      assert (well_typed (G' & x ~ T') (e & x ~ v)) by auto.
-      assert (x \notin L0) by auto.
-      inversion Hlc.
-
-      apply (proj1 (lc_at_to_open_trm_val_def_defs x)) in H14.
-      specialize (H0 _ H3 H14 H5 (G' & x ~ T') H7 H8 (e & x ~ v) H9 _ (H6 _ H10)).
-      apply_fresh ty_let as y; eauto.
-
-      apply weaken_ty_trm with (G2:=(y ~ T')) in H0; auto.
-
-      pose proof (proj1 (subst_rules y T')) as Hsubst.
-      specialize (Hsubst _ _ _ H0 G' (y ~ T') x).
-      assert (HsubstU : subst_typ x y U = U). {
-        apply subst_fresh_typ. auto.
-      }
-
-      assert (Hxyt : subst_typ x y T' = T'). {
-        apply subst_fresh_typ. auto.
-      }
-
-      assert (Hopeny : subst_ctx x y (y ~ T') = y ~ T'). {
-        unfold subst_ctx. rewrite map_single, Hxyt. trivial.
-      }
-
-      assert (Hopent : subst_trm x y (open_trm x t'0) = open_trm y t'0). {
-        rewrite subst_open_commut_trm.
-        rewrite (proj1 (subst_fresh_trm_val_def_defs _ _)); auto.
-        unfold subst_fvar. case_if; auto.
-      }
-      rewrite HsubstU, Hopeny, Hopent in Hsubst.
-
-      apply Hsubst; auto.
-      rewrite Hxyt; auto.
-
-  - apply narrow_typing with (G' := G') in Ht; auto.
-    apply narrow_subtyping with (G' := G') in H; auto.
-    eauto.
+    destruct t; try solve [solve_let].
+    + SCase "[t = (let x = a in u)] where a is a variable".
+      repeat invert_red.
+      exists (@empty typ). rewrite concat_empty_r. repeat split; auto.
+      lets Hok: (well_typed_to_ok_G Hwf). apply* renaming_fresh.
+    + SCase "[t = (let x = v in u)] where v is a value".
+      repeat invert_red.
+      match goal with
+        | [Hn: ?x # ?s |- _] =>
+          pose proof (well_typed_notin_dom Hwf Hn) as Hng
+      end.
+      pose proof (val_typing Ht) as [V [Hv Hs]].
+      exists (x ~ V). repeat split.
+      ** rewrite <- concat_empty_l. constructor~. apply (precise_inert_typ Hv).
+      ** constructor~. apply (precise_to_general Hv).
+      ** eapply renaming_fresh with (L:=L \u dom G \u \{x}). apply* ok_push.
+         intros. apply* weaken_rules. apply ty_sub with (T:=V); auto. apply* weaken_subtyp.
+  - Case "ty_sub".
+    solve_IH.
+    match goal with
+    | [Hs: _ ⊢ _ <: _,
+       Hg: _ & ?G' ⊢ _: _ |- _] =>
+      apply weaken_subtyp with (G2:=G') in Hs;
+      eauto
+    end.
 Qed.
 
+(** ** Preservation Theorem *)
 
-(** ** Preservation Theorem
-    If [⊢ t : T] and [t |-> t'], then [⊢ t': T]. *)
-Theorem preservation: forall (t t' : trm) T,
-    lc_trm t ->
-    ⊢ t: T ->
-    t |-> t' ->
-    ⊢ t' : T.
+(** [⊢ (s, t): T]           #<br>#
+    [(s, t) |-> (s', t')]   #<br>#
+    [―――――――――――――――――――]   #<br>#
+    [⊢ (s', t'): T]         *)
+Theorem preservation : forall s s' t t' T,
+    ⊢ (s, t) : T ->
+    (s, t) |-> (s', t') ->
+    ⊢ (s', t') : T.
 Proof.
-  intros. eapply preservation_ec; eauto.
+  introv Ht Hr. destruct Ht as [* Hi Hwf Ht].
+  lets Hp: (preservation_helper Hwf Hi Hr Ht). destruct Hp as [G' [Hi' [Hwf' Ht']]].
+  apply sta_trm_typ_c with (G:=G & G'); auto. apply* inert_concat.
+Qed.
+
+(** * Progress *)
+
+(** Helper tactic for proving progress *)
+Ltac solve_let_prog :=
+  match goal with
+      | [IH: ⊢ (?s, ?t) : ?T ->
+             inert _ ->
+             well_typed _ _ -> _,
+         Hi: inert _,
+         Hwt: well_typed _ _ |- _] =>
+        assert (⊢ (s, t): T) as Hs by eauto;
+        specialize (IH Hs Hi Hwt) as [IH | [s' [t' Hr]]];
+        eauto; inversion IH
+      end.
+
+(** ** Progress Theorem *)
+
+(** [⊢ (s, t): T]           #<br>#
+    [(s, t) |-> (s', t')]   #<br>#
+    [―――――――――――――――――――]   #<br>#
+    [t] is in normal form   #<br>#
+    or [exists s', t'] such that [(s, t) |-> (s', t')] *)
+Theorem progress: forall s t T,
+    ⊢ (s, t) : T ->
+    norm_form t \/ exists s' t', (s, t) |-> (s', t').
+Proof.
+  introv Ht. inversion Ht as [G s' t' T' Hi Hwt HT]. subst.
+  induction HT; eauto.
+  - Case "ty_all_elim".
+    pose proof (canonical_forms_fun Hi Hwt HT1). destruct_all. right*.
+  - Case "ty_new_elim".
+    pose proof (canonical_forms_obj Hi Hwt HT). destruct_all. right*.
+  - Case "ty_let".
+    right. destruct t; try solve [solve_let_prog].
+    + pose proof (var_typing_implies_avar_f HT) as [x A]. subst*.
+    + pick_fresh x. exists (s & x ~ v) (open_trm x u). auto.
 Qed.
