src/extensions/paths-new/Substitution.v
@@ -8,408 +8,7 @@ Set Implicit Arguments.
 
 Require Import List Coq.Program.Equality.
 Require Import LibLN.
-Require Import Definitions Weakening Binding.
-
-(** * Definitions *)
-
-(** Substitution on variables: [a[u/z]] (substituting [z] with [u] in [a]). *)
-(*
-Definition subst_var (z: var) (u: var) (x: var): var :=
-  If x = z then u else x.
-
-Definition subst_var_p (z: var) (u: path) (x: var): path :=
-  If x = z then u else (pvar x).
-
-Hint Unfold subst_var subst_var_p.
-
-Definition subst_avar (z: var) (u: path) (a: avar) : path :=
-  match a with
-  | avar_b i => p_sel (avar_b i) nil
-  | avar_f x => subst_var_p z u x
-  end.
-
-(* p    [u / z] where p = x.bs:
-   x.bs [u / z] == x [u / z] . bs *)
-Definition subst_path (z: var) (u: path) (p: path) : path :=
-  match p with
-  | p_sel x bs => sel_fields (subst_avar z u x) bs
-  end.
-
-(** Substitution on types and declarations: [T[u/z]] and [D[u/z]]. *)
-Fixpoint subst_typ (z: var) (u: path) (T: typ) { struct T } : typ :=
-  match T with
-  | typ_top        => typ_top
-  | typ_bot        => typ_bot
-  | typ_rcd D      => typ_rcd (subst_dec z u D)
-  | typ_and T1 T2  => typ_and (subst_typ z u T1) (subst_typ z u T2)
-  | typ_path q L    => typ_path (subst_path z u q) L
-  | typ_bnd T      => typ_bnd (subst_typ z u T)
-  | typ_all T U    => typ_all (subst_typ z u T) (subst_typ z u U)
-  end
-with subst_dec (z: var) (u: path) (D: dec) { struct D } : dec :=
-  match D with
-  | dec_typ L T U => dec_typ L (subst_typ z u T) (subst_typ z u U)
-  | dec_trm L U => dec_trm L (subst_typ z u U)
-  end.
-
-(** Substitution on terms, values, and definitions:
-    [t[u/z]], [v[u/z]], [d[u/z]]. *)
-Fixpoint subst_trm (z: var) (u: path) (t: trm) : trm :=
-  match t with
-  | trm_val v        => trm_val (subst_val z u v)
-  | trm_path p       => trm_path (subst_path z u p)
-  | trm_app x1 x2    => trm_app (subst_path z u x1) (subst_path z u x2)
-  | trm_let t1 t2    => trm_let (subst_trm z u t1) (subst_trm z u t2)
-  end
-with subst_val (z: var) (u: path) (v: val) : val :=
-  match v with
-  | val_new T ds     => val_new (subst_typ z u T) (subst_defs z u ds)
-  | val_lambda T t   => val_lambda (subst_typ z u T) (subst_trm z u t)
-  end
-with subst_def (z: var) (u: path) (d: def) : def :=
-  match d with
-  | def_typ L T => def_typ L (subst_typ z u T)
-  | def_trm L t => def_trm L (subst_trm z u t)
-  end
-with subst_defs (z: var) (u: path) (ds: defs) : defs :=
-  match ds with
-  | defs_nil => defs_nil
-  | defs_cons rest d => defs_cons (subst_defs z u rest) (subst_def z u d)
-  end.
-
-(** Substitution on the types of a typing environment: [G[u/z]]. *)
-Definition subst_ctx (z: var) (u: path) (G: ctx) : ctx :=
-  map (subst_typ z u) G.
-
-(** * Lemmas *)
-
-(** The following [subst_fresh_XYZ] lemmas state that if [x] is not free
-    in a symbol [Y], then [Y[z/x] = Y]. *)
-
-(** Fresh substitution
-    - in variables *)
-Lemma subst_fresh_avar: forall x y,
-  (forall a: avar, x \notin fv_avar a -> subst_avar x y a = p_sel a nil).
-Proof.
-  intros. destruct* a. simpl. autounfold. case_var*. simpls. notin_false.
-Qed.
-
-Lemma subst_fresh_path : forall x q p,
-    x \notin fv_path p ->
-    subst_path x q p = p.
-Proof.
-  intros. destruct p as [[n | z] bs]; simpls.
-  - Case "p = (avar_b n).bs".
-    rewrite* app_nil_r.
-  - Case "p = (avar_f z).bs".
-    unfold subst_var_p. apply notin_singleton in H. case_if.
-    simpl. rewrite* app_nil_r.
-Qed.
-
-(** - in types, declarations, paths *)
-Lemma subst_fresh_typ_dec: forall x y,
-  (forall T : typ  , x \notin fv_typ  T  -> subst_typ  x y T  = T ) /\
-  (forall D : dec  , x \notin fv_dec  D  -> subst_dec  x y D  = D ).
-Proof.
-  intros x y. apply typ_mutind; intros; simpls; f_equal*. apply* subst_fresh_path.
-Qed.
-
-Definition subst_fresh_typ x p := proj1 (subst_fresh_typ_dec x p).
-
-(** - in terms, values, and definitions *)
-Lemma subst_fresh_trm_val_def_defs: forall x y,
-  (forall t : trm , x \notin fv_trm  t  -> subst_trm  x y t  = t ) /\
-  (forall v : val , x \notin fv_val  v  -> subst_val  x y v  = v ) /\
-  (forall d : def , x \notin fv_def  d  -> subst_def  x y d  = d ) /\
-  (forall ds: defs, x \notin fv_defs ds -> subst_defs x y ds = ds).
-Proof.
-  intros x y. apply trm_mutind; intros; simpls; f_equal*;
-    (apply* subst_fresh_typ_dec || apply* subst_fresh_path).
-Qed.
-
-Lemma fv_ctx_types_push_eq : forall G x T,
-    fv_ctx_types (G & x ~ T) = fv_ctx_types G \u fv_typ T.
-Proof.
-  intros.
-  rewrite concat_def, single_def.
-  unfold fv_ctx_types, fv_in_values; rewrite values_def.
-  rewrite union_comm. simpl. reflexivity.
-Qed.
-
-Lemma fv_ctx_types_concat_eq : forall G1 G2,
-    fv_ctx_types (G1 & G2) = fv_ctx_types G1 \u fv_ctx_types G2.
-Proof.
-  intros G1 G2. induction G2 using env_ind.
-  - unfold fv_ctx_types, fv_in_values; rewrite values_def.
-    rewrite concat_empty_r, empty_def, union_empty_r; reflexivity.
-  - rewrite concat_assoc. rewrite fv_ctx_types_push_eq.
-    rewrite IHG2. rewrite <- union_assoc. f_equal.
-    symmetry. apply fv_ctx_types_push_eq.
-Qed.
-
-Lemma notin_fv_ctx_concat : forall x G2 G1,
-    x \notin fv_ctx_types (G1 & G2) <->
-    x \notin fv_ctx_types G1 /\ x \notin fv_ctx_types G2.
-Proof.
-  intros. rewrite <- notin_union.
-  rewrite <- fv_ctx_types_concat_eq.
-  split; intros; assumption.
-Qed.
-
-(** [x \notin fv(T)]           #<br>#
-    [x \notin fv(G)]       #<br>#
-    [―――――――――――――――――――――――] #<br>#
-    [x \notin fv(G, z: T)] *)
-Lemma fv_ctx_types_push: forall x z T G,
-    x \notin fv_typ T ->
-    x \notin fv_ctx_types G ->
-    x \notin fv_ctx_types (G & z ~ T).
-Proof.
-  intros. rewrite fv_ctx_types_push_eq.
-  apply notin_union. split~.
-Qed.
-
-(** [x \notin fv(G, z: T)]                   #<br>#
-    [x \notin fv(T)]                         #<br>#
-    [―――――――――――――――――――――――――――――――――――――] #<br>#
-    [x \notin fv(T)] and [x \notin fv(G)] *)
-Lemma invert_fv_ctx_types_push: forall x z T G,
-  x \notin fv_ctx_types (G & z ~ T) -> x \notin fv_typ T /\ x \notin (fv_ctx_types G).
-Proof.
-  introv H. rewrite fv_ctx_types_push_eq in H.
-  apply~ notin_union.
-Qed.
-
-(** [x \notin fv(G)]         #<br>#
-    [――――――――――――――――――]    #<br>#
-    [G[y/x] = G]    *)
-Lemma subst_fresh_ctx: forall x y G,
-  x \notin fv_ctx_types G -> subst_ctx x y G = G.
-Proof.
-  intros x y.
-  apply (env_ind (fun G => x \notin fv_ctx_types G -> subst_ctx x y G = G)).
-  + intro N. unfold subst_ctx. apply map_empty.
-  + intros G z T IH N.
-    apply invert_fv_ctx_types_push in N. destruct N as [N1 N2].
-    unfold subst_ctx in *. rewrite map_push.
-    rewrite (IH N2).
-    rewrite ((proj1 (subst_fresh_typ_dec _ _)) _ N1).
-    reflexivity.
-Qed.
-(*
-(** Definition of substitution on named variables: #<br>#
-    [z[y/x] := if z == x then y else z], where [z] is a named variable. *)
-Definition subst_fvar(x y z: var): var := If z = x then y else z.*)
-
-(** The following lemmas state that substitution commutes with opening:
-    for a symbol [Z], #<br>#
-    [(Z^a)[y/x] = (Z[y/x])^(a[y/x])]. *)
-
-(** Substitution commutes with opening
-    - variables *)
-Lemma subst_open_commut: forall x p u y n,
-    lc_path p ->
-    subst_avar x p (open_rec_avar n u y)
-    = open_rec_path_p n (subst_var_p x p u) (subst_avar x p y).
-Proof.
-  introv Hl. unfold subst_var_p, subst_avar, open_rec_avar, subst_var_p.
-  destruct y as [n' | y]; autounfold; destruct p as [z bs]; destruct z as [m | z'];
-    repeat case_if; simpl; try case_if*; eauto; inversions  Hl; inversions H0.
-Qed.
-
-Lemma sel_fields_open : forall n p q bs,
-  sel_fields (open_rec_path_p n p q) bs = open_rec_path_p n p (sel_fields q bs).
-Proof.
-  intros. destruct q. simpl. destruct p. destruct a. case_if; simpl; auto. rewrite* app_assoc.
-  simpl. auto.
-Qed.
-
-Lemma sel_fields_subst : forall x p y bs b,
-    subst_path x p (p_sel y bs) • b = (subst_path x p (p_sel y bs)) • b.
-Proof.
-  intros. destruct p, y; auto. simpl. unfold subst_var_p. case_if; simpl; auto.
-Qed.
-
-(** - paths *)
-Lemma subst_open_commut_path: forall p n x q u,
-    lc_path p ->
-    subst_path x p (open_rec_path n u q)
-    = open_rec_path_p n (subst_var_p x p u) (subst_path x p q).
-Proof.
-  introv Hl. destruct q as [z bs]. simpl. rewrite* subst_open_commut. rewrite* sel_fields_open.
-Qed.
-
-(** - types and declarations *)
-Lemma subst_open_commut_typ_dec: forall x p u,
-  lc_path p ->
-  (forall t : typ, forall n: nat,
-     subst_typ x p (open_rec_typ n u t)
-     = open_rec_typ_p n (subst_var_p x p u) (subst_typ x p t)) /\
-  (forall D : dec, forall n: nat,
-     subst_dec x p (open_rec_dec n u D)
-     = open_rec_dec_p n (subst_var_p x p u) (subst_dec x p D)).
-Proof.
-  intros. apply typ_mutind; intros; simpl; f_equal*. apply* subst_open_commut_path.
-Qed.
-
-Lemma subst_open_commut_p: forall x p u y n,
-    lc_path p ->
-    subst_path x p (open_rec_avar_p n u y)
-    = open_rec_path_p n (subst_path x p u) (subst_avar x p y).
-Proof.
-  introv Hl. unfold subst_path, subst_avar, subst_var_p.
-  destruct y as [n' | y]; simpl; repeat case_if; destruct u; destruct a; simpl;
-    try (rewrite* app_nil_r); repeat case_if; unfold sel_fields; destruct* p;
-      inversions Hl; inversions H0; rewrite* app_nil_l.
-Qed.
-
-Lemma subst_open_commut_path_p: forall p n x q u,
-    lc_path q ->
-    subst_path x q (open_rec_path_p n u p)
-    = open_rec_path_p n (subst_path x q u) (subst_path x q p).
-Proof.
-  introv Hl. destruct p as [z bs]. simpl.
-  unfold subst_path. destruct u. rewrite <- sel_fields_open.
-  unfold open_rec_path_p, subst_avar.
-  destruct z; simpl; destruct a; repeat case_if*;
-    unfold subst_var_p; repeat case_if;
-      destruct q; simpl; try (rewrite app_assoc || rewrite app_nil_r);
-        try solve [inversion Hl; inversion* H0].
-Qed.
-
-Lemma subst_open_commut_typ_dec_p: forall x y u,
-  lc_path y ->
-  (forall t : typ, forall n: nat,
-     subst_typ x y (open_rec_typ_p n u t)
-     = open_rec_typ_p n (subst_path x y u) (subst_typ x y t)) /\
-  (forall D : dec, forall n: nat,
-     subst_dec x y (open_rec_dec_p n u D)
-     = open_rec_dec_p n (subst_path x y u) (subst_dec x y D)).
-Proof.
-  intros. apply typ_mutind; intros; simpl; f_equal*.
-  apply* subst_open_commut_path_p.
-Qed.
-
-(** - types only *)
-Lemma subst_open_commut_typ: forall x y u T,
-  lc_path y ->
-  subst_typ x y (open_typ u T) = open_typ_p (subst_var_p x y u) (subst_typ x y T).
-Proof.
-  intros. apply* subst_open_commut_typ_dec.
-Qed.
-
-Lemma subst_open_commut_typ_p: forall x y u T,
-    lc_path y ->
-    subst_typ x y (open_typ_p u T) = open_typ_p (subst_path x y u) (subst_typ x y T).
-Proof.
-  intros. apply* subst_open_commut_typ_dec_p.
-Qed.
-
-(** - terms, values, definitions, and list of definitions *)
-Lemma subst_open_commut_trm_val_def_defs: forall x y u,
-    lc_path y ->
-  (forall t : trm, forall n: nat,
-     subst_trm x y (open_rec_trm n u t)
-     = open_rec_trm_p n (subst_var_p x y u) (subst_trm x y t)) /\
-  (forall v : val, forall n: nat,
-     subst_val x y (open_rec_val n u v)
-     = open_rec_val_p n (subst_var_p x y u) (subst_val x y v)) /\
-  (forall d : def , forall n: nat,
-     subst_def x y (open_rec_def n u d)
-     = open_rec_def_p n (subst_var_p x y u) (subst_def x y d)) /\
-  (forall ds: defs, forall n: nat,
-     subst_defs x y (open_rec_defs n u ds)
-     = open_rec_defs_p n (subst_var_p x y u) (subst_defs x y ds)).
-Proof.
-  intros. apply trm_mutind; intros; simpl; f_equal*;
-  apply* subst_open_commut_path || apply* subst_open_commut_typ_dec.
-Qed.
-
-Lemma subst_open_commut_trm_val_def_defs_p: forall x y u,
-    lc_path y ->
-  (forall t : trm, forall n: nat,
-     subst_trm x y (open_rec_trm_p n u t)
-     = open_rec_trm_p n (subst_path x y u) (subst_trm x y t)) /\
-  (forall v : val, forall n: nat,
-     subst_val x y (open_rec_val_p n u v)
-     = open_rec_val_p n (subst_path x y u) (subst_val x y v)) /\
-  (forall d : def , forall n: nat,
-     subst_def x y (open_rec_def_p n u d)
-     = open_rec_def_p n (subst_path x y u) (subst_def x y d)) /\
-  (forall ds: defs, forall n: nat,
-     subst_defs x y (open_rec_defs_p n u ds)
-     = open_rec_defs_p n (subst_path x y u) (subst_defs x y ds)).
-Proof.
-  intros. apply trm_mutind; intros; simpl; f_equal*;
-  apply* subst_open_commut_typ_dec_p || apply* subst_open_commut_path_p.
-Qed.
-
-(** - terms only *)
-Lemma subst_open_commut_trm: forall x y u t,
-    lc_path y ->
-    subst_trm x y (open_trm u t)
-    = open_trm_p (subst_var_p x y u) (subst_trm x y t).
-Proof.
-  intros. apply* subst_open_commut_trm_val_def_defs.
-Qed.
-
-Lemma subst_open_commut_trm_p: forall x y u t,
-    lc_path y ->
-    subst_trm x y (open_trm_p u t)
-    = open_trm_p (subst_path x y u) (subst_trm x y t).
-Proof.
-  intros. apply* subst_open_commut_trm_val_def_defs_p.
-Qed.
-
-(** - definitions only *)
-Lemma subst_open_commut_defs: forall x y u ds,
-    lc_path y ->
-    subst_defs x y (open_defs u ds)
-    = open_defs_p (subst_var_p x y u) (subst_defs x y ds).
-Proof.
-  intros. apply* subst_open_commut_trm_val_def_defs.
-Qed.
-
-Lemma subst_open_commut_defs_p: forall x y u ds,
-    lc_path y ->
-    subst_defs x y (open_defs_p u ds)
-    = open_defs_p (subst_path x y u) (subst_defs x y ds).
-Proof.
-  intros. apply* subst_open_commut_trm_val_def_defs_p.
-Qed.
-
-(** The following lemmas state that opening a symbol with a variable [y]
-    is the same as opening the symbol with another variable [x] and
-    substituting [x] with [y]: #<br>#
-    [Z^y = (Z^x)[y/x]] *)
-
-(** Substitution after opening
-    - terms *)
-Lemma subst_intro_trm: forall x u t, x \notin (fv_trm t) -> lc_path u ->
-  open_trm_p u t = subst_trm x u (open_trm x t).
-Proof.
-  introv Fr Hl. unfold open_trm. rewrite* subst_open_commut_trm.
-  destruct (@subst_fresh_trm_val_def_defs x u) as [Q _]. rewrite~ (Q t).
-  unfold subst_var_p. case_var~.
-Qed.
-
-(** - definitions *)
-Lemma subst_intro_defs: forall x u ds, x \notin (fv_defs ds) -> lc_path u ->
-  open_defs_p u ds = subst_defs x u (open_defs x ds).
-Proof.
-  introv Fr Hl. unfold open_trm. rewrite* subst_open_commut_defs.
-  destruct (@subst_fresh_trm_val_def_defs x u) as [_ [_ [_ Q]]]. rewrite~ (Q ds).
-  unfold subst_var_p. case_var~.
-Qed.
-
-(** - types *)
-Lemma subst_intro_typ: forall x u T, x \notin (fv_typ T) -> lc_path u ->
-  open_typ_p u T = subst_typ x u (open_typ x T).
-Proof.
-  introv Fr Hl. unfold open_typ. rewrite* subst_open_commut_typ.
-  destruct (@subst_fresh_typ_dec x u) as [Q _]. rewrite* (Q T).
-  unfold subst_var_p. case_var*.
-Qed.
+Require Import Definitions Binding Weakening.
 
 Ltac subst_open_fresh :=
   match goal with
@@ -423,25 +22,6 @@ Ltac subst_open_fresh :=
         replace (open_trm z (subst_trm x p t)) with (open_trm_p (subst_path x p (pvar z)) (subst_trm x p t))
           by (unfold subst_path; simpl; unfold subst_var_p; rewrite If_r, open_var_trm_eq; auto)
     end.
-
-(** Substitution preserves labels of definitions: [label(d) = label(d[y/x])] *)
-Lemma subst_label_of_def: forall x y d,
-  label_of_def d = label_of_def (subst_def x y d).
-Proof.
-  intros. destruct* d.
-Qed.
-
-(** [l \notin labels(ds)]     #<br>#
-    [――――――――――――――――――――――] #<br>#
-    [l \notin labels(ds[y/x]] *)
-Lemma subst_defs_hasnt: forall x y l ds,
-  defs_hasnt ds l ->
-  defs_hasnt (subst_defs x y ds) l.
-Proof.
-  intros x y l ds. unfold defs_hasnt. induction ds; introv Eq; auto.
-  unfold get_def. simpl. rewrite <- subst_label_of_def.
-  simpl in Eq. case_if~.
-Qed.*)
 
 Ltac subst_fresh_solver :=
   fresh_constructor;
@@ -626,48 +206,59 @@ Proof.
     unfold subst_ctx in *; try rewrite map_empty in *; try rewrite concat_empty_r in *; auto.
 Qed.
 
-Lemma renaming_def: forall G z T ds x P,
+(** * Renaming  *)
+
+(** Renaming the name of the opening variable for definition typing.  #<br>#
+
+    [ok G]                   #<br>#
+    [z] fresh                #<br>#
+    [G, z: T^z ⊢ ds^z : T^z] #<br>#
+    [――――――――――――――――――――――] #<br>#
+    [G ⊢ ds^x : T^x]         *)
+Lemma renaming_def: forall G z T ds x,
     ok G ->
     z # G ->
-    z \notin fv_ctx_types G \u fv_defs ds \u fv_typ T ->
-    z; nil; P; G & z ~ open_typ z T ⊢ open_defs z ds :: open_typ z T ->
-    G ⊢ tvar x : open_typ x T ->
-    x; nil; P; G ⊢ open_defs x ds :: open_typ x T.
+    z \notin (fv_ctx_types G \u fv_defs ds \u fv_typ T) ->
+    G & z ~ open_typ z T /- open_defs z ds :: open_typ z T ->
+    G ⊢ trm_var (avar_f x) : open_typ x T ->
+    G /- open_defs x ds :: open_typ x T.
 Proof.
-  introv Hok Hnz Hnz' Hz Hx. rewrite open_var_typ_eq.
-  assert (lc_path (pvar x)) as Hl by constructor*.
-  rewrite subst_intro_typ with (x:=z); auto. rewrite open_var_defs_eq.
-  rewrite subst_intro_defs with (x:=z); auto.
-  assert (x = subst_var z x z) as Hxz by (unfold subst_var; case_if*).
-  rewrite Hxz at 1. eapply subst_ty_defs; auto. eapply Hz. unfold pvar. eauto. rewrite <- subst_intro_typ; auto.
-  rewrite* <- open_var_typ_eq. case_if*.
+  introv Hok Hnz Hnz' Hz Hx. rewrite subst_intro_typ with (x:=z). rewrite subst_intro_defs with (x:=z).
+  eapply subst_ty_defs; auto. eapply Hz. rewrite <- subst_intro_typ. all: auto.
 Qed.
 
-Lemma renaming_def': forall G z T ds x bs P,
-    ok G ->
-    x # G ->
-    x \notin (fv_ctx_types G \u fv_defs ds \u fv_typ T) ->
-    z; bs; P; G ⊢ open_defs_p (p_sel (avar_f z) bs) ds :: open_typ_p (p_sel (avar_f z) bs) T ->
-    G ⊢ trm_path (p_sel (avar_f z) bs) : open_typ_p (p_sel (avar_f z) bs) T ->
-    x; nil; P; G & x ~ open_typ x T ⊢ open_defs x ds :: open_typ x T.
-Proof.
-  introv Hok Hx Hx' Hds Hp.
-  assert (lc_path (p_sel (avar_f z) bs)) as Hl by constructor*.
-  apply weaken_ty_defs with (G2:=x ~ open_typ x T) in Hds; auto.
-  apply weaken_ty_trm with (G2:= x ~ open_typ x T) in Hp; auto. Admitted. (*
-  lets Hpr: (proj43 (path_replacement T Hl)). eapply Hpr in Hds; eauto.
-Qed.*)
-
+(** Renaming the name of the opening variable for term typing. #<br>#
+    [ok G]                   #<br>#
+    [z] fresh                #<br>#
+    [G, z: U ⊢ t^z : T^z]    #<br>#
+    [――――――――――――――――――――――] #<br>#
+    [G ⊢ t^x : T^x]         *)
 Lemma renaming_typ: forall G z T U t x,
     ok G ->
     z # G ->
-    lc_path (pvar x) ->
     z \notin (fv_ctx_types G \u fv_typ U \u fv_typ T \u fv_trm t) ->
     G & z ~ U ⊢ open_trm z t : open_typ z T ->
-    G ⊢ tvar x : U ->
+    G ⊢ trm_var (avar_f x) : U ->
     G ⊢ open_trm x t : open_typ x T.
 Proof.
-  introv Hok Hnz Hl Hnz' Hz Hx. rewrite open_var_trm_eq. rewrite open_var_typ_eq.
-  rewrite subst_intro_typ with (x:=z). rewrite subst_intro_trm with (x:=z).
-  eapply subst_ty_trm; eauto. rewrite~ subst_fresh_typ. all: auto.
+  introv Hok Hnz Hnz' Hz Hx. rewrite subst_intro_typ with (x:=z). rewrite subst_intro_trm with (x:=z).
+  eapply subst_ty_trm; auto. eapply Hz. rewrite subst_fresh_typ. all: auto.
+Qed.
+
+(** Renaming the name of the opening variable for term typing. #<br>#
+    [ok G]                   #<br>#
+    [z] fresh                #<br>#
+    [G, z: U ⊢ t^z : T^z]    #<br>#
+    [――――――――――――――――――――――] #<br>#
+    [G ⊢ t^x : T^x]         *)
+Lemma renaming_fresh : forall L G T u U x,
+    ok G ->
+    (forall x : var, x \notin L -> G & x ~ T ⊢ open_trm x u : U) ->
+    G ⊢ trm_var (avar_f x) : T ->
+    G ⊢ open_trm x u : U.
+Proof.
+  introv Hok Hu Hx. pick_fresh y.
+  rewrite subst_intro_trm with (x:=y); auto.
+  rewrite <- subst_fresh_typ with (x:=y) (y:=x); auto.
+  eapply subst_ty_trm; eauto. rewrite~ subst_fresh_typ.
 Qed.
