src/extensions/paths-new/RecordAndInertTypes.v
@@ -1,0 +1,298 @@
+(** printing ⊢#    %\vdash_{\#}%    #&vdash;<sub>&#35;</sub>#     *)
+(** printing ⊢##   %\vdash_{\#\#}%  #&vdash;<sub>&#35&#35</sub>#  *)
+(** printing ⊢##v  %\vdash_{\#\#v}% #&vdash;<sub>&#35&#35v</sub># *)
+(** printing ⊢!    %\vdash_!%       #&vdash;<sub>!</sub>#         *)
+(** remove printing ~ *)
+
+Set Implicit Arguments.
+
+Require Import LibLN.
+Require Import Coq.Program.Equality.
+Require Import Definitions Binding.
+
+(** * Record Types *)
+
+(** ** Lemmas About Records and Record Types *)
+
+(** [G |- ds :: U]                          #<br>#
+    [U] is a record type with labels [ls]  #<br>#
+    [ds] are definitions with label [ls']  #<br>#
+    [l \notin ls']                          #<br>#
+    [―――――――――――――――――――――――――――――――――――]  #<br>#
+    [l \notin ls] *)
+Lemma hasnt_notin : forall x bs P G ds ls l U,
+    x; bs; P; G ⊢ ds :: U ->
+    record_typ U ls ->
+    defs_hasnt ds l ->
+    l \notin ls.
+Proof.
+
+  Ltac inversion_def_typ :=
+    match goal with
+    | H: _; _; _; _ ⊢ _ : _ |- _ => inversions H
+    end.
+
+  introv Hds Hrec Hhasnt.
+  inversions Hhasnt. gen ds. induction Hrec; intros; inversions Hds.
+  - inversion_def_typ; simpl in *; case_if; apply* notin_singleton.
+  - apply notin_union; split; simpl in *.
+    + apply* IHHrec. case_if*.
+    + inversion_def_typ; case_if; apply* notin_singleton.
+Qed.
+
+(** [labels(D) = labels(D^x)] *)
+Lemma open_dec_preserves_label: forall D x i,
+  label_of_dec D = label_of_dec (open_rec_dec i x D).
+Proof.
+  intros. induction D; reflexivity.
+Qed.
+
+Lemma open_dec_preserves_label_p: forall D p i,
+  label_of_dec D = label_of_dec (open_rec_dec_p i p D).
+Proof.
+  intros. induction D; simpl; reflexivity.
+Qed.
+
+Lemma open_record:
+  (forall D, record_dec D ->
+        forall x k, record_dec (open_rec_dec k x D)) /\
+  (forall T ls , record_typ T ls ->
+        forall x k, record_typ (open_rec_typ k x T) ls) /\
+  (forall T, inert_typ T ->
+        forall x k, inert_typ (open_rec_typ k x T)).
+Proof.
+  apply rcd_mutind; intros; try constructor; auto;
+    try solve [erewrite open_dec_preserves_label in e; eauto].
+  unfold open_typ. simpl. eauto.
+Qed.
+
+Lemma open_record_p:
+  (forall D, record_dec D ->
+        forall p k, record_dec (open_rec_dec_p k p D)) /\
+  (forall T ls , record_typ T ls ->
+        forall p k, record_typ (open_rec_typ_p k p T) ls) /\
+  (forall T, inert_typ T ->
+        forall p k, inert_typ (open_rec_typ_p k p T)).
+Proof.
+  apply rcd_mutind; intros; try constructor; auto;
+    try solve [erewrite open_dec_preserves_label_p in e; eauto].
+  unfold open_typ. simpl. eauto.
+Qed.
+
+(** [record_dec D]   #<br>#
+    [――――――――――――――] #<br>#
+    [record_dec D^x] *)
+Lemma open_record_dec: forall D x,
+  record_dec D -> record_dec (open_dec x D).
+Proof.
+  intros. apply* open_record.
+Qed.
+
+Lemma open_record_dec_p: forall D x,
+  record_dec D -> record_dec (open_dec_p x D).
+Proof.
+  intros. apply* open_record_p.
+Qed.
+
+(** [record_typ T]   #<br>#
+    [――――――――――――――] #<br>#
+    [record_typ T^x] *)
+Lemma open_record_typ: forall T x ls,
+  record_typ T ls -> record_typ (open_typ x T) ls.
+Proof.
+  intros. apply* open_record.
+Qed.
+
+Lemma open_record_typ_p: forall T p ls,
+  record_typ T ls -> record_typ (open_typ_p p T) ls.
+Proof.
+  intros. apply* open_record_p.
+Qed.
+
+(** [record_typ T]   #<br>#
+    [――――――――――――――] #<br>#
+    [record_typ T^x] *)
+Lemma open_record_type: forall T x,
+  record_type T -> record_type (open_typ x T).
+Proof.
+  intros. destruct H as [ls H]. exists ls. eapply open_record_typ.
+  eassumption.
+Qed.
+
+Lemma open_record_type_p: forall T p,
+  record_type T -> record_type (open_typ_p p T).
+Proof.
+  intros. destruct H as [ls H]. exists ls. eapply open_record_typ_p.
+  eassumption.
+Qed.
+
+(** The type of definitions is a record type. *)
+Lemma ty_defs_record_type : forall z bs P G ds T,
+    z; bs; P; G ⊢ ds :: T ->
+    record_type T.
+Proof.
+  intros. induction H; destruct D;
+    repeat match goal with
+        | [ H: record_type _ |- _ ] =>
+          destruct H
+        | [ Hd: _; _; _; _ ⊢ _ : { _ >: _ <: _ } |- _ ] =>
+          inversions Hd
+        | [ Hd: _; _; _; _ ⊢ _ : dec_trm _ _  |- _ ] =>
+          inversions Hd
+    end;
+    match goal with
+    | [ ls: fset label,
+        t: trm_label |- _ ] =>
+      exists (ls \u \{ label_trm t })
+    | [ ls: fset label,
+        t: typ_label |- _ ] =>
+      exists (ls \u \{ label_typ t })
+    | [ t: trm_label |- _ ] =>
+      exists \{ label_trm t }
+    | [ t: typ_label |- _ ] =>
+      exists \{ label_typ t }
+    end;
+    constructor*; try constructor; apply (hasnt_notin H); eauto.
+Qed.
+
+(** Opening does not affect the labels of a [record_typ]. *)
+Lemma opening_preserves_labels : forall z T ls ls',
+    record_typ T ls ->
+    record_typ (open_typ z T) ls' ->
+    ls = ls'.
+Proof.
+  introv Ht Hopen. gen ls'.
+  dependent induction Ht; intros.
+  - inversions Hopen. rewrite* <- open_dec_preserves_label.
+  - inversions Hopen. rewrite* <- open_dec_preserves_label.
+    specialize (IHHt ls0 H4). rewrite* IHHt.
+Qed.
+
+ Ltac invert_open :=
+    match goal with
+    | [ H: _ = open_rec_typ _ _ ?T' |- _ ] =>
+       destruct T'; inversions* H
+    | [ H: _ = open_rec_dec _ _ ?D' |- _ ] =>
+       destruct D'; inversions* H
+    end.
+
+Lemma record_open:
+  (forall D, record_dec D ->
+        forall x k D',
+          x \notin fv_dec D' ->
+          D = open_rec_dec k x D' ->
+          record_dec D') /\
+  (forall T ls , record_typ T ls ->
+            forall x k T',
+              x \notin fv_typ T' ->
+              T = open_rec_typ k x T' ->
+              record_typ T' ls) /\
+  (forall T, inert_typ T ->
+        forall x k T',
+          x \notin fv_typ T' ->
+          T = open_rec_typ k x T' ->
+          inert_typ T').
+Proof.
+  apply rcd_mutind; intros; invert_open; simpls.
+  - apply open_fresh_typ_dec_injective in H4; auto. subst. constructor.
+  - constructor*. rewrite* <- open_dec_preserves_label.
+  - invert_open. simpls. constructor*. rewrite* <- open_dec_preserves_label.
+Qed.
+
+(** If [T] is a record type with labels [ls], and [T = ... /\ D /\ ...],
+    then [label(D) isin ls]. *)
+Lemma record_typ_has_label_in: forall T D ls,
+  record_typ T ls ->
+  record_has T D ->
+  label_of_dec D \in ls.
+Proof.
+  introv Htyp Has. generalize dependent D. induction Htyp; intros.
+  - inversion Has. subst. apply in_singleton_self.
+  - inversion Has; subst; rewrite in_union.
+    + left. apply* IHHtyp.
+    + right. inversions H5. apply in_singleton_self.
+Qed.
+
+(** [T = ... /\ {A: T1..T1} /\ ...] #<br>#
+    [T = ... /\ {A: T2..T2} /\ ...] #<br>#
+    [―――――――――――――――――――――――――――] #<br>#
+    [T1 = T2] *)
+Lemma unique_rcd_typ: forall T A T1 T2,
+  record_type T ->
+  record_has T (dec_typ A T1 T1) ->
+  record_has T (dec_typ A T2 T2) ->
+  T1 = T2.
+Proof.
+  introv Htype Has1 Has2.
+  generalize dependent T2. generalize dependent T1. generalize dependent A.
+  destruct Htype as [ls Htyp]. induction Htyp; intros; inversion Has1; inversion Has2; subst.
+  - inversion* H3.
+  - inversion* H5.
+  - apply record_typ_has_label_in with (D:=dec_typ A T1 T1) in Htyp.
+    + inversions H9. false* H1.
+    + assumption.
+  - apply record_typ_has_label_in with (D:=dec_typ A T2 T2) in Htyp.
+    + inversions H5. false* H1.
+    + assumption.
+  - inversions H5. inversions* H9.
+Qed.
+
+Lemma unique_rcd_trm: forall T a U1 U2,
+    record_type T ->
+    record_has T (dec_trm a U1) ->
+    record_has T (dec_trm a U2) ->
+    U1 = U2.
+Proof.
+  introv Htype Has1 Has2.
+  gen U1 U2 a.
+  destruct Htype as [ls Htyp]. induction Htyp; intros; inversion Has1; inversion Has2; subst.
+  - inversion* H3.
+  - inversion* H5.
+  - eapply record_typ_has_label_in with (D:=dec_trm a U1) in Htyp.
+    + inversions H9. false* H1.
+    + assumption.
+  - apply record_typ_has_label_in with (D:=dec_trm a U2) in Htyp.
+    + inversions H5. false* H1.
+    + inversions H5. lets Hr: (record_typ_has_label_in Htyp H9).
+      false* H1.
+  - inversions H5. inversions* H9.
+Qed.
+
+(** [ds = ... /\ {a = t} /\ ...]  #<br>#
+    [ds = ... /\ {a = t'} /\ ...] #<br>#
+    [―――――――――――――――――――――――――] #<br>#
+    [t = t'] *)
+Lemma defs_has_inv: forall ds a t t',
+    defs_has ds (def_trm a t) ->
+    defs_has ds (def_trm a t') ->
+    t = t'.
+Proof.
+  intros. unfold defs_has in *.
+  inversions H. inversions H0.
+  rewrite H1 in H2. inversions H2.
+  reflexivity.
+Qed.
+
+Lemma record_has_sel_typ: forall G p T a U,
+    G ⊢ trm_path p : T ->
+    record_has T (dec_trm a U) ->
+    G ⊢ trm_path (p • a) : U.
+Proof.
+  introv Hp Hr. dependent induction Hr; eauto.
+Qed.
+
+Lemma inert_concat: forall G' G,
+     inert G ->
+     inert G' ->
+     ok (G & G') ->
+     inert (G & G').
+ Proof.
+   induction G' using env_ind; introv Hg Hg' Hok.
+   - rewrite* concat_empty_r.
+   - rewrite concat_assoc.
+     inversions Hg'; inversions Hok;
+       rewrite concat_assoc in *; try solve [false* empty_push_inv].
+     destruct (eq_push_inv H) as [Heq1 [Heq2 Heq3]]; subst.
+     destruct (eq_push_inv H3) as [Heq1 [Heq2 Heq3]]; subst.
+     apply inert_all; auto.
+ Qed.
