README.md
@@ -11,8 +11,8 @@ This repo contains:
 - the [simple DOT safety proof](https://github.com/amaurremi/dot-calculus/tree/master/src/simple-proof)
 - extensions of DOT with:
   * mutation (adding _mutable references_ to DOT)
-  ([proof](https://github.com/amaurremi/dot-calculus/tree/master/src/mutation) | [technical report](https://arxiv.org/abs/1611.07610))
+  ([proof](https://github.com/amaurremi/dot-calculus/tree/master/src/extensions/mutation) | [technical report](https://arxiv.org/abs/1611.07610))
   * expanded type paths (adding type selections on _full paths_ of the form `p.A` instead of `x.A`, where `p` is a path and `x` is a variable)
-  ([proof in progress](https://github.com/amaurremi/dot-calculus/tree/master/src/paths))
+  ([proof in progress](https://github.com/amaurremi/dot-calculus/tree/master/src/extensions/paths))
   * initialization order (developing a sound _initialization order_)
-  ([proof in progress](https://github.com/amaurremi/dot-calculus/tree/master/src/initialization))
+  ([proof in progress](https://github.com/amaurremi/dot-calculus/tree/master/src/extensions/initialization))
